theories/lib/int.v
@@ -4,12 +4,34 @@ From iris_c.lib Require Export prelude Integers.
 Require Import iris.prelude.prelude.
 From mathcomp Require Export ssreflect.
 
-Definition op_safe op (i j: nat) : Prop :=
-    Z.to_nat (Byte.intval (op (Byte.repr i) (Byte.repr j))) = i * j.
+Definition op_safe op opn (i j: nat) : Prop :=
+    Z.to_nat (Byte.intval (op (Byte.repr i) (Byte.repr j))) = opn i j.
 
-Definition mul_safe := op_safe Byte.mul.
+Definition mul_safe := op_safe Byte.mul Init.Nat.mul.
 
 Coercion Byte.repr : Z >-> int8.
+
+Global Instance int_eq_dec : EqDecision int.
+Proof. apply Int.eq_dec. Defined.
+Global Instance byte_eq_dec : EqDecision byte.
+Proof. apply Byte.eq_dec. Defined.
+Global Instance int8_eq_dec : EqDecision int8.
+Proof. apply Byte.eq_dec. Defined.
+Global Instance int32_eq_dec: EqDecision int32 := Int.eq_dec.
+
+Definition int8_encode (i: int8) : positive := encode (Byte.unsigned i).
+Definition int8_decode (p: positive) : option int8 :=
+  match decode p with
+    | Some z => Some (Byte.repr z)
+    | None => None
+  end.
+
+Lemma int8_decode_encode i: int8_decode (int8_encode i) = Some i.
+Proof. unfold int8_encode, int8_decode. rewrite decode_encode.
+       f_equal. apply Byte.repr_unsigned. Qed.
+
+Global Instance int8_countable: Countable int8 :=
+  Build_Countable _ _ int8_encode int8_decode int8_decode_encode.
 
 Bind Scope int_scope with int.
 Delimit Scope int_scope with int.
