theories/tests/rec.v
@@ -5,54 +5,85 @@ Section proof.
   Context `{clangG Σ}.
 
   Definition f : expr :=
-    if: ("x" != 0)
+    if: (!"x"@Tint8 != 0)
     then: (
-      "x" <- "x" - 1 ;;
+      "x" <- !"x"@Tint8 - 1 ;;
       Ecall Tvoid "g" (Epair (Evar "x") (Evalue Vvoid)) ;;
       return: void)
     else: ( return: void ).
 
   Definition g : expr :=
-    if: ("x" != 0)
+    if: (!"x"@Tint8 != 0)
     then: (
-      "x" <- "x" - 1 ;;
+      "x" <- !"x"@Tint8 - 1 ;;
       Ecall Tvoid "f" (Epair (Evar "x") (Evalue Vvoid));;
       return: void)
     else: ( return: void ).
 
-  Lemma rec_example (n: nat) k ks Φ:
-    "f" T↦ Function Tvoid [("x", Tint8)] f ∗
-    "g" T↦ Function Tvoid [("x", Tint8)] g ∗ Φ void
+  Definition rec_env n : env := (sset "x" (Tptr Tint8, Vptr n) semp).
+
+  Definition Pn : Prop :=
+    (∀ n: nat, Byte.repr n = ((Z.pos (Pos.of_succ_nat n) - 1%Z)%int)) ∧
+    (∀ n: nat, evalbop oneq (Z.pos (Pos.of_succ_nat n)) 0%Z = Some vtrue).
+  
+  Lemma rec_example (ln: addr) (n: nat) k ks Φ:
+    Pn →
+    ln ↦ n @ Tint8 ∗
+    "f" T↦ Function Tvoid [("x", Tptr Tint8)] f ∗
+    "g" T↦ Function Tvoid [("x", Tptr Tint8)] g ∗ (WP (fill_ectxs void k, ks) {{ Φ }})
     ⊢ WP (fill_ectxs (Ecall Tvoid "f"
-                            (Evalue (Vpair (Vint8 n) Vvoid))) k, ks) {{ Φ }}.
+                            (Evalue (Vpair ln void))) k, ks) {{ Φ }}.
   Proof.
-    iIntros "[#? [#? HΦ]]".
-    iLöb as "IH" forall (n k ks Φ).
-    destruct n eqn:?; subst.
-    - admit. (* simple base case *)
-    - (* iApply (wp_call _ (Vpair (Vint8 (S n0)) Vvoid)); last iFrame "#"; first done. *)
-      (* iNext. wp_alloc ln as "Hln". *)
-      (* wp_let. wp_load. wp_op. *)
-      (* { instantiate (1:=vtrue). admit. } *)
-      (* wp_step. iNext. wp_load. wp_op. *)
-      (* replace (Z.pos (Pos.of_succ_nat n0) - 1%Z)%int with (Int.repr n0); last admit. *)
-      (* wp_assign. *)
-      (* iApply (wp_bind [EKseq _; EKcall _ _])=>//. *)
-      (* admit. *)
-      (* wp_load. iApply wp_value=>//. *)
-      (* wp_unfill (Ecall _ _ _). *)
-      (* iApply (wp_call [EKseq (return: void)] [Vint32 n0]); *)
-      (*   last iFrame "#"; first done. *)
-      (* iNext. wp_alloc lx as "Hlx". *)
-      (* wp_let. wp_load. *)
-      (* destruct n0 eqn:?; subst. *)
-      (* + admit. *)
-      (* + replace (S n != 0%Z)%E with (Evalue vtrue); last admit. *)
-      (*   do 5 wp_step. wp_unfill (Ecall _ _ _)%E. *)
-      (*   simpl. *)
-      (*   replace (! lx @ Tint32)%E with *)
-      (*   (Evalue $ (n - 1)); last admit. wp_unfill (Ecall _ _ _)%E. *)
-      (*   iApply ("IH" $! (n - 1)). done. *)
-  Admitted.
-    
+    iIntros (Hn) "[Hn [#? [#? HΦ]]]".
+    iLöb as "IH" forall (n k ks Φ Hn). destruct ks.
+    iApply (wp_call (rec_env ln) e _ (Vpair ln Vvoid) [("x", Tptr Tint8)])=>//.
+    destruct n eqn:?; subst; iFrame "#"; iNext.
+    - unfold f. wp_var. by wp_run.
+    - unfold f. wp_var. wp_run=>//.
+      { destruct Hn as [H1 H2].
+        specialize H2 with n0. done. }
+      wp_step. iNext. wp_var. wp_var. wp_run.
+      wp_unfill (Ecall _ _ _).
+      rewrite (fill_app (Evar "x")
+                        [EKcall Tvoid "g"; EKpairl void]).
+      iApply wp_bind=>//.
+      wp_var. iApply wp_value=>//.
+      wp_unfill (Ecall _ _ _).
+      rewrite (fill_app (Epair ln void)
+                        [EKcall Tvoid "g"]).
+      iApply wp_bind=>//. wp_pair.
+      iApply wp_value=>//.
+      replace ((Z.pos (Pos.of_succ_nat n0) - 1%Z)%int)
+        with (Byte.repr n0).
+      iApply (wp_call (rec_env ln) (rec_env ln) [EKseq (return: void)]
+                      (Vpair ln void));
+        last iFrame "#"; first done.
+      iNext. unfold g. wp_var. wp_load.
+      destruct n0 eqn:Heqn; subst.
+      + wp_run. simpl. wp_run. done.
+      + simpl.
+        wp_op=>//.
+        { destruct Hn as [H1 H2]. simpl. apply H2. }
+        wp_step. iApply wp_seq=>//. iNext. wp_var. wp_var. wp_run.
+        wp_unfill (Ecall _ _ _)%E.
+        rewrite (fill_app (Evar "x")
+                          [EKcall Tvoid "f"; EKpairl void]).
+        iApply wp_bind=>//.
+        wp_var. iApply wp_value=>//.
+        wp_unfill (Ecall _ _ _).
+        rewrite (fill_app (Epair ln void) [EKcall Tvoid "f"]).
+        iApply wp_bind=>//. wp_pair.
+        iApply wp_value=>//.
+        wp_unfill (Ecall _ _ _).
+        replace (Z.pos (Pos.of_succ_nat n) - 1%Z)%int
+        with (Byte.repr n).
+        iDestruct ("IH" $! n) as "IH'".
+        iDestruct ("IH'" $! _ _ _ with "[]") as "?"=>//.
+        iApply ("~2" with "[-HΦ]")=>//.
+        simpl. wp_run. simpl. wp_run.
+        { by destruct Hn as [? ?]. }
+        { by destruct Hn as [? ?]. }
+      + destruct Hn as [? ?]. done.
+  Qed.
+
 End proof.
