theories/clang/lib/vmm.v
@@ -3,17 +3,17 @@ Require Import iris_c.clang.lib.page_table.
 Require Import iris_c.lib.int.
 
 Section vmm.
-  Context `{clangG Σ} {pt: page_table Σ}.
+  Context `{G: clangG Σ} {pt: @page_table Σ G}.
 
   Definition mem_init (n: nat) (x: addr) (y: addr) : expr :=
     x <- 0 ;;
-    while: ( !x@Tint32 :<: n ) (
+    while: ( !x@Tint8 :<: n ) (
       y <- Ealloc (Tprod Tint8 Tvoid) (Vpair vfalse Vvoid) ;;
-      Ecall Tvoid (insert_pt pt) (Epair (!x@Tint32) (Evalue (Vpair (Vptr y) Vvoid)))
+      Ecall Tvoid (insert_pt pt) (Epair (!x@Tint8) (Evalue (Vpair (Vptr y) Vvoid)))
     ).
 
-  Fixpoint allocated (m: gmap int32 addr) (n: nat) : iProp Σ :=
-    match m !! Int.repr n with
+  Fixpoint allocated (m: gmap int8 addr) (n: nat) : iProp Σ :=
+    match m !! Byte.repr n with
       | None => False%I
       | Some p =>
         (p ↦ (Vpair vfalse Vvoid) @ (Tprod Tint8 Tvoid) ∗
@@ -22,10 +22,5 @@ Section vmm.
              | S n' => allocated m n'
         end)%I
       end.
-
-  Lemma mem_init_spec n x y ks Φ:
-    is_page_table pt ∅ ∗ (∀ m, allocated m (n - 1) -∗ is_page_table pt m -∗ Φ Vvoid)
-    ⊢ WP (mem_init n x y, ks) {{ Φ }}.
-  Admitted.
 
 End vmm.
