theories/clang/memory.v
@@ -1,5 +1,5 @@
 (** Definition of the physical memory model **)
-From iris_c.lib Require Import Coqlib.
+From iris_c.lib Require Import Coqlib int.
 Require Export Integers.
 Require Export iris.base_logic.base_logic.
 
@@ -19,10 +19,6 @@ Definition shift_loc l (o: nat) : addr :=
 
 Instance addr_eq_dec : EqDecision addr.
 Proof. solve_decision. Defined.
-Instance int_eq_dec : EqDecision int.
-Proof. apply Int.eq_dec. Defined.
-Instance byte_eq_dec : EqDecision byte.
-Proof. apply Byte.eq_dec. Defined.
 
 (* Byte-level value *)
 Inductive byteval : Set :=
@@ -36,7 +32,6 @@ Inductive val : Set :=
 | Vvoid
 | Vnull
 | Vint8 (i: int8)
-(* | Vint32 (i: int32) *)
 | Vptr (p: addr)
 | Vpair (v1 v2: val).
 
@@ -51,7 +46,6 @@ Instance sizeof_val: Sizeof val :=
     | Vnull => 4 %nat
     | Vvoid => 0 % nat
     | Vint8 _ => 1 % nat
-    (* | Vint32 _ => 4 % nat *)
     | Vptr _ => 4 % nat
     | Vpair v1 v2 => (go v1 + go v2)%nat
   end.
@@ -135,7 +129,6 @@ Definition proj_pointer (vl: list byteval) : option val :=
 
 Fixpoint encode_val (v: val) : list byteval :=
   match v with
-    (* | Vint32 n => inj_bytes (encode_int 4%nat (Int.unsigned n)) *)
     | Vint8 n => inj_bytes (encode_int 1%nat (Byte.unsigned n))
     | Vptr p => inj_pointer 4%nat p
     | Vnull => list_repeat 4 BVnull
